theories/core/utp_expr.thy
@@ -1,0 +1,420 @@
+(******************************************************************************)
+(* Project: Unifying Theories of Programming in HOL                           *)
+(* File: utp_pred.thy                                                         *)
+(* Author: Simon Foster and Frank Zeyda, University of York (UK)              *)
+(******************************************************************************)
+
+header {* Basic Expressions *}
+
+theory utp_expr
+imports  utp_pred utp_unrest utp_sorts
+begin
+
+text {* The type which an expression holds should be the maximal type, if such a notion exists *}
+type_synonym ('VALUE, 'TYPE) EXPRESSION = "('TYPE * ('VALUE, 'TYPE) BINDING_FUN)"
+
+context PRED
+begin
+
+definition expr_type :: "('VALUE, 'TYPE) EXPRESSION \<Rightarrow> 'TYPE" ("\<tau>e") where
+"expr_type e = fst e"
+
+definition expr_bfun :: "('VALUE, 'TYPE) EXPRESSION \<Rightarrow> ('VALUE, 'TYPE) BINDING_FUN" where
+"expr_bfun = snd"
+
+lemma expr_simps [simp]:
+  "expr_bfun (t,f) = f"
+  "expr_type (t,f) = t"
+  by (simp_all add:expr_type_def expr_bfun_def)
+
+definition etype_rel :: "('VALUE, 'TYPE) EXPRESSION \<Rightarrow> 'TYPE \<Rightarrow> bool" (infix ":e:" 50) where
+"etype_rel e t \<equiv> \<forall>b\<in>WF_BINDING. expr_bfun e b : t"
+
+definition UNREST_EXPR :: "('TYPE VAR) set \<Rightarrow> ('VALUE, 'TYPE) EXPRESSION \<Rightarrow> bool" where
+"UNREST_EXPR vs f \<equiv> (\<forall> b1 \<in> WF_BINDING . \<forall> b2 \<in> WF_BINDING . expr_bfun f (b1 \<oplus> b2 on vs) = expr_bfun f b1)" 
+
+text {* A well-formed expression must produce a well-typed value for every binding, and non well-formed bindings yield an fixed arbitrary well-typed value *}
+
+definition WF_EXPRESSION :: "('VALUE, 'TYPE) EXPRESSION set" where
+"WF_EXPRESSION = {f. \<forall>b. if (b \<in> WF_BINDING) then expr_bfun f b : (expr_type f) else expr_bfun f b = default (expr_type f)}"
+
+definition WF_EXPRESSION_OVER ::
+  "('TYPE VAR) set \<Rightarrow>
+   ('VALUE, 'TYPE) EXPRESSION set" where
+"WF_EXPRESSION_OVER vs = {e . e \<in> WF_EXPRESSION \<and> UNREST_EXPR (VAR - vs) e}"
+
+subsection {* Operators *}
+
+subsubsection {* Well-formed expression builders *}
+
+definition wfexpr ::
+"('VALUE, 'TYPE) EXPRESSION \<Rightarrow> 
+ ('VALUE, 'TYPE) EXPRESSION" where
+"wfexpr f \<equiv> (expr_type f, \<lambda> b. if (b \<in> WF_BINDING) then expr_bfun f b else default (expr_type f))"
+
+subsubsection {* Equality *}
+
+definition EqualP :: 
+"('VALUE, 'TYPE) EXPRESSION \<Rightarrow> 
+ ('VALUE, 'TYPE) EXPRESSION \<Rightarrow> 
+ ('VALUE, 'TYPE) PREDICATE" where
+"e \<in> WF_EXPRESSION \<and> f \<in> WF_EXPRESSION \<longrightarrow>
+EqualP e f = {b \<in> WF_BINDING. expr_bfun e b = expr_bfun f b}"
+
+notation EqualP (infixr "==p" 200)
+
+definition VarE :: "'TYPE VAR \<Rightarrow> ('VALUE, 'TYPE) EXPRESSION" where
+"VarE x \<equiv> wfexpr (type x, \<lambda> b. b x)"
+
+definition LitE :: "'TYPE \<Rightarrow> 'VALUE \<Rightarrow> ('VALUE, 'TYPE) EXPRESSION" where
+"LitE t v \<equiv> wfexpr (t, \<lambda> b. v)"
+
+definition DefaultE :: "'TYPE \<Rightarrow> ('VALUE, 'TYPE) EXPRESSION" where
+"DefaultE t \<equiv> LitE t (default t)"
+
+definition SubstE :: 
+"('VALUE, 'TYPE) EXPRESSION \<Rightarrow> 
+ ('VALUE, 'TYPE) EXPRESSION \<Rightarrow> 
+ 'TYPE VAR \<Rightarrow> 
+ ('VALUE, 'TYPE) EXPRESSION" ("_[_|_]" [200]) where
+"f \<in> WF_EXPRESSION \<and> v \<in> WF_EXPRESSION \<longrightarrow>
+SubstE f v x = wfexpr (expr_type f, \<lambda> b. expr_bfun f (b(x := expr_bfun v b)))"
+
+definition SubstPE ::
+"('VALUE, 'TYPE) PREDICATE \<Rightarrow> 
+ ('VALUE, 'TYPE) EXPRESSION \<Rightarrow> 
+ 'TYPE VAR \<Rightarrow> 
+ ('VALUE, 'TYPE) PREDICATE" ("_[_|_]" [200]) where
+"p[v|x] \<equiv> (\<exists>p {x} . p \<and>p (VarE x ==p v))"
+
+subsection {* Theorems *}
+
+subsubsection {* Well-formed expression properties *}
+
+lemma WF_EXPRESSION_bfun [simp]:
+  "e \<in> WF_EXPRESSION \<Longrightarrow> expr_bfun e b : expr_type e"
+  apply (simp add:WF_EXPRESSION_def, case_tac "b \<in> WF_BINDING")
+  apply (simp_all add:default_type)
+done
+
+lemma EXPRESSION_eqI [intro]:
+  "\<lbrakk> expr_type e = expr_type f; \<forall> b. expr_bfun e b = expr_bfun f b \<rbrakk> \<Longrightarrow>
+  e = f"
+  by (case_tac e, case_tac f, auto)
+
+(* It would be nice to have this as a typing rule, but it
+   confuses the HO unifier... *)
+
+theorem WF_EXPRESSION_type: 
+"\<lbrakk> e \<in> WF_EXPRESSION; e :e: t; b \<in> WF_BINDING \<rbrakk> \<Longrightarrow>
+expr_bfun e b : t"
+  by (simp add:WF_EXPRESSION_def etype_rel_def)
+
+theorem WF_EXPRESSION_has_type [typing]: 
+"\<lbrakk> e \<in> WF_EXPRESSION \<rbrakk> \<Longrightarrow> \<exists> t. e :e: t"
+  apply (rule_tac x="expr_type e" in exI)
+  apply (auto simp add: etype_rel_def)
+done
+
+theorem WF_EXPRESSION_default [simp]:
+"\<lbrakk> e \<in> WF_EXPRESSION; b \<notin> WF_BINDING \<rbrakk> \<Longrightarrow>
+ expr_bfun e b = default (expr_type e)"
+  by (auto simp add:WF_EXPRESSION_def)
+
+theorem WF_EXPRESSION_wfexpr_bfun [simp]:
+"\<lbrakk> b \<in> WF_BINDING \<rbrakk> \<Longrightarrow> expr_bfun (wfexpr e) b = expr_bfun e b"
+  by (simp add:wfexpr_def)
+
+lemma WF_EXPRESSION_value_exists:
+  "e \<in> WF_EXPRESSION \<Longrightarrow> \<forall> b. \<exists> v. v : \<tau>e e \<and> expr_bfun e b = v"
+  apply (case_tac e)
+  apply (auto simp add:WF_EXPRESSION_def LitE_def wfexpr_def)
+  apply (case_tac "ba \<in> WF_BINDING")
+  apply (drule_tac x="ba" in spec)
+  apply (simp)
+  apply (drule_tac x="ba" in spec)
+  apply (simp add:default_type)
+done
+
+lemma WF_EXPRESSION_value_elim [elim]:
+  "\<lbrakk> e \<in> WF_EXPRESSION;
+     \<And> v b. \<lbrakk> v : \<tau>e e; expr_bfun e b = v \<rbrakk> \<Longrightarrow> P \<rbrakk> \<Longrightarrow>
+   P"
+  by (metis WF_EXPRESSION_bfun)
+ 
+subsubsection {* Closure Theorems *}
+
+theorem WF_EXPRESSION_wfexpr [closure]:
+"e :e: expr_type e \<Longrightarrow> wfexpr e \<in> WF_EXPRESSION"
+  by (unfold WF_EXPRESSION_def wfexpr_def, auto simp add:etype_rel_def)
+
+
+theorem WF_EXPRESSION_BODY_wfexpr_drop [simp]:
+"e \<in> WF_EXPRESSION \<Longrightarrow> wfexpr e = e"
+  apply (rule EXPRESSION_eqI)
+  apply (simp_all add:WF_EXPRESSION_def wfexpr_def)
+done
+
+theorem wfexpr_idem [simp]: "wfexpr (wfexpr e) = wfexpr e"
+  by (auto simp add: wfexpr_def)
+
+theorem EqualP_closure[closure]: "\<lbrakk> e \<in> WF_EXPRESSION; f \<in> WF_EXPRESSION \<rbrakk> \<Longrightarrow> e ==p f \<in> WF_PREDICATE"
+  by (auto intro:closure simp add:EqualP_def WF_EXPRESSION_def WF_PREDICATE_def WF_BINDING_def)
+
+theorem VarE_closure[closure]: "VarE x \<in> WF_EXPRESSION"
+  by (auto intro!:closure simp add:VarE_def closure WF_BINDING_def etype_rel_def)
+
+theorem LitE_closure[closure]: 
+assumes "v : t"
+shows "LitE t v \<in> WF_EXPRESSION"
+  by (auto intro:closure simp add:LitE_def WF_BINDING_def etype_rel_def assms)
+ 
+theorem DefaultE_closure[closure]:
+"DefaultE t \<in> WF_EXPRESSION"
+  by (simp add:DefaultE_def closure default_type)
+
+theorem SubstE_closure[closure]:
+ assumes "e \<in> WF_EXPRESSION" "v \<in> WF_EXPRESSION" "v :e: type x"
+ shows "(e::('VALUE,'TYPE) EXPRESSION)[v|x] \<in> WF_EXPRESSION"
+  by (auto intro:closure simp add:SubstE_def WF_BINDING_def etype_rel_def assms)
+
+theorem SubstPE_closure[closure]:
+ assumes "p \<in> WF_PREDICATE" "v \<in> WF_EXPRESSION" "v :e: type x"
+ shows "SubstPE p v x \<in> WF_PREDICATE"
+  by (simp add:SubstPE_def closure assms)
+
+subsubsection {* Typing Theorems *}
+
+theorem expr_type [typing]: "e \<in> WF_EXPRESSION \<Longrightarrow> e :e: \<tau>e e"
+  by (simp add:etype_rel_def)
+
+theorem wfexpr_tau [simp]: "\<tau>e (wfexpr e) = \<tau>e e"
+  by (simp add:wfexpr_def)
+
+theorem VarE_type [typing]: "VarE x :e: type x"
+  by (simp add:VarE_def WF_BINDING_def typing etype_rel_def)
+
+theorem VarE_tau [simp]: "\<tau>e (VarE x) = type x"
+  by (simp add:VarE_def)
+
+theorem LitE_type [typing]: 
+"v : t \<Longrightarrow> LitE t v :e: t"
+  by (simp add:LitE_def etype_rel_def typing)
+
+theorem LitE_tau [simp]:
+"\<tau>e (LitE t e) = t"
+  by (simp add:LitE_def)
+
+theorem DefaultE_type [typing]:
+"DefaultE t :e: t"
+  by (simp add:DefaultE_def typing)
+
+theorem DefaultE_tau [typing]:
+"\<tau>e (DefaultE t) = t"
+  by (simp add:DefaultE_def)
+
+theorem SubstE_type [typing]:
+"\<lbrakk> e \<in> WF_EXPRESSION; v \<in> WF_EXPRESSION; v :e: type x; e :e: t \<rbrakk> \<Longrightarrow>
+ e[v|x] :e: t"
+  by (simp add:SubstE_def etype_rel_def WF_BINDING_update1)
+
+theorem SubstE_tau [simp]:
+"\<lbrakk>e \<in> WF_EXPRESSION; v \<in> WF_EXPRESSION\<rbrakk> \<Longrightarrow> \<tau>e (SubstE e v x) = \<tau>e e"
+  by (simp add:SubstE_def)
+
+subsubsection {* @{term UNREST_EXPR} Theorems *}
+
+theorem UNREST_EXPR_member [unrest] :
+"\<lbrakk>f \<in> WF_EXPRESSION; 
+ UNREST_EXPR vs f;
+ b \<in> WF_BINDING;
+ b' \<in> WF_BINDING\<rbrakk> \<Longrightarrow>
+ expr_bfun f b = expr_bfun f (b \<oplus> b' on vs)"
+  apply (simp only:WF_EXPRESSION_def)
+  apply (unfold UNREST_EXPR_def)
+  apply (erule_tac x="b" in ballE)
+  apply (erule_tac x="b'" in ballE)
+  apply (auto)
+done
+
+theorem UNREST_EXPR_empty [unrest] :
+"e \<in> WF_EXPRESSION \<Longrightarrow> UNREST_EXPR {} e"
+  by (simp add: UNREST_EXPR_def)
+
+theorem UNREST_EXPR_subset [unrest] :
+"\<lbrakk>UNREST_EXPR vs1 e;
+ vs2 \<subseteq> vs1;
+ e \<in> WF_EXPRESSION\<rbrakk> \<Longrightarrow>
+ UNREST_EXPR vs2 e"
+  apply (simp add:UNREST_EXPR_def)
+  apply (clarify)
+  apply (subgoal_tac "expr_bfun e b1 = expr_bfun e (b1 \<oplus> b2 on vs1)")
+  apply (drule_tac x = "b1 \<oplus> b2 on vs2" in bspec)
+  apply (simp add:closure)
+  apply (drule_tac x = "b2" in bspec)
+  apply (simp add:closure)
+  apply (simp add:override_on_assoc)
+  apply (subgoal_tac "vs2 \<union> vs1 = vs1")
+  apply (auto)
+done
+
+theorem UNREST_EqualP [unrest] :
+"\<lbrakk> e \<in> WF_EXPRESSION; f \<in> WF_EXPRESSION;
+ UNREST_EXPR vs1 e; UNREST_EXPR vs2 f \<rbrakk> \<Longrightarrow>
+ UNREST (vs1 \<inter> vs2) (e ==p f)"
+  apply (auto simp add:EqualP_def)
+  apply (drule_tac ?vs2.0="vs1 \<inter> vs2" in UNREST_EXPR_subset)
+  apply (simp_all)
+  apply (drule_tac ?vs2.0="vs1 \<inter> vs2" in UNREST_EXPR_subset)
+  apply (simp_all)
+  apply (simp add:UNREST_EXPR_def UNREST_def)
+  apply (safe)
+  apply (rule closure)
+  apply (simp_all)
+done
+
+theorem UNREST_EXPR_wfexpr [unrest]:
+"UNREST_EXPR vs e \<Longrightarrow> UNREST_EXPR vs (wfexpr e)"
+  by (simp add:wfexpr_def UNREST_EXPR_def closure)
+
+theorem UNREST_EXPR_VarE [unrest] :
+"UNREST_EXPR (vs - {x}) (VarE x)"
+  apply (simp add:VarE_def)
+  apply (rule unrest)
+  apply (simp add:UNREST_EXPR_def)
+done
+
+theorem UNREST_EXPR_LitE [unrest] :
+"UNREST_EXPR vs (LitE t v)"
+  apply (simp add:LitE_def)
+  apply (rule unrest)
+  apply (simp add:UNREST_EXPR_def)
+done
+
+theorem UNREST_EXPR_SubstE [unrest] :
+"\<lbrakk> f \<in> WF_EXPRESSION; v \<in> WF_EXPRESSION; v :e: type x;
+   UNREST_EXPR vs1 f; UNREST_EXPR vs2 v \<rbrakk> \<Longrightarrow>
+ UNREST_EXPR ((vs1 \<union> {x}) \<inter> vs2) (f[v|x])"
+apply (subgoal_tac "UNREST_EXPR (vs1 \<inter> vs2) f")
+apply (subgoal_tac "UNREST_EXPR ((vs1 \<union> {x}) \<inter> vs2) v")
+apply (subgoal_tac "UNREST_EXPR ((vs1 \<union> {x}) \<inter> vs2 - {x}) f")
+apply (simp add:SubstE_def)
+apply (rule unrest)
+apply (simp add:UNREST_EXPR_def)
+apply (clarify)
+apply (subgoal_tac "b1(x := expr_bfun v b1) \<in> WF_BINDING")
+apply (simp)
+apply (simp add:etype_rel_def closure)
+apply (force intro:UNREST_EXPR_subset)+
+done
+
+end
+
+subsection {* Boolean Expressions *}
+
+context PRED_BOOL
+begin
+
+definition TrueE :: "('VALUE, 'TYPE) EXPRESSION" where
+"TrueE \<equiv> LitE BoolType (MkBool True)"
+
+definition FalseE :: "('VALUE, 'TYPE) EXPRESSION" where
+"FalseE \<equiv> LitE BoolType (MkBool False)"
+
+definition ExprP :: "('VALUE, 'TYPE) EXPRESSION \<Rightarrow> ('VALUE, 'TYPE) PREDICATE" where
+"ExprP e = LiftP (DestBool \<circ> expr_bfun e)"
+
+definition PredE :: "('VALUE, 'TYPE) PREDICATE \<Rightarrow> ('VALUE, 'TYPE) EXPRESSION" where
+"p \<in> WF_PREDICATE \<longrightarrow> 
+PredE p = wfexpr (BoolType, \<lambda> b. MkBool (b \<in> p))"
+
+definition VarP ::  "'TYPE VAR \<Rightarrow> ('VALUE, 'TYPE) PREDICATE" where
+"VarP v \<equiv> LiftP (DestBool \<circ> expr_bfun (VarE v))"
+
+subsubsection {* Closure Theorems *}
+
+theorem TrueE_closed [closure]: "TrueE \<in> WF_EXPRESSION"
+  by (auto intro:closure typing simp add:TrueE_def)
+
+theorem FalseE_closed [closure]: "FalseE \<in> WF_EXPRESSION"
+  by (auto intro:closure typing simp add:FalseE_def)
+
+theorem ExprP_closed [closure]: 
+"ExprP e \<in> WF_PREDICATE"
+  by (simp add: ExprP_def closure)
+
+theorem PredE_closed [closure]: "p \<in> WF_PREDICATE \<Longrightarrow> PredE p \<in> WF_EXPRESSION"
+  apply (simp add:PredE_def)
+  apply (rule closure)
+  apply (simp add:etype_rel_def typing)
+done
+
+theorem VarP_closed [closure]: "VarP x \<in> WF_PREDICATE"
+  by (simp add:VarP_def, rule closure)
+
+subsubsection {* Typing Theorems *}
+
+theorem TrueE_type [typing]: "TrueE :e: BoolType"
+  apply (simp add: TrueE_def)
+  apply (rule typing)+
+done
+
+theorem FalseE_type [typing]: "FalseE :e: BoolType"
+  apply (simp add: FalseE_def)
+  apply (rule typing)+
+done
+
+theorem PredE_type [typing]:
+"p \<in> WF_PREDICATE \<longrightarrow>
+PredE p :e: BoolType"
+  by (auto intro:typing simp add:PredE_def etype_rel_def)
+
+subsubsection {* Laws about booleans *}
+
+lemma notext [elim]: "\<lbrakk> f \<noteq> g; \<And> x. f x \<noteq> g x \<Longrightarrow> P \<rbrakk> \<Longrightarrow> P"
+  by (auto)
+
+ 
+lemma ExprP_TrueE [simp]: "ExprP TrueE = true"
+  by (simp add:ExprP_def TrueE_def LiftP_def expr_bfun_def LitE_def wfexpr_def TrueP_def)
+
+lemma ExprP_FalseE [simp]: "ExprP FalseE = false"
+  by (simp add:ExprP_def FalseE_def LiftP_def expr_bfun_def LitE_def wfexpr_def FalseP_def)
+
+
+subsubsection {* @{term UNREST_EXPR} Theorems *}
+
+theorem UNREST_EXPR_TrueE [unrest]: "UNREST_EXPR vs TrueE"
+  by (simp add:TrueE_def unrest)
+
+theorem UNREST_EXPR_FalseE [unrest]: "UNREST_EXPR vs FalseE"
+  by (simp add:FalseE_def unrest)
+
+theorem UNREST_ExprP [unrest]:
+"\<lbrakk> e \<in> WF_EXPRESSION; UNREST_EXPR vs e; e :e: BoolType \<rbrakk> \<Longrightarrow> UNREST vs (ExprP e)"
+  apply (simp add:ExprP_def)
+  apply (rule unrest)
+  oops
+
+theorem UNREST_EXPR_PredE [unrest]: 
+"\<lbrakk>p \<in> WF_PREDICATE; UNREST vs p\<rbrakk> \<Longrightarrow> UNREST_EXPR vs (PredE p)"
+  apply (simp add:PredE_def)
+  apply (rule unrest)
+  apply (simp add:UNREST_EXPR_def UNREST_def WF_PREDICATE_def)
+  apply (safe)
+  apply (rule_tac f="MkBool" and g="MkBool" in cong, simp)
+  apply (auto)
+  apply (metis override_on_cancel1 override_on_cancel2)
+done
+  
+theorem UNREST_VarP [unrest]:
+"UNREST (vs - {x}) (VarP x)"
+apply (simp add:VarP_def)
+apply (rule_tac ?vs1.0="{x}" in UNREST_LiftP_alt)
+apply (auto)
+apply (simp add:WF_BINDING_PRED_def VarE_def wfexpr_def binding_equiv_def) 
+done
+
+
+end
+end
