theories/tactics/utp_alpha_expr_tac.thy
@@ -1,0 +1,99 @@
+(******************************************************************************)
+(* Project: Unifying Theories of Programming                                  *)
+(* File: utp_alpha_expr_tac.thy                                               *)
+(* Author: Simon Foster and Frank Zeyda, University of York (UK)              *)
+(******************************************************************************)
+
+header {* Proof Tactic for Alphabetised Expressions *}
+
+theory utp_alpha_expr_tac
+imports "../alpha/utp_alpha_expr" utp_pred_tac utp_expr_tac utp_alpha_tac
+begin
+
+context ALPHA_PRED
+begin
+
+subsection {* Interpretation Function *}
+
+definition EvalAE ::
+  "('VALUE, 'TYPE) ALPHA_EXPRESSION \<Rightarrow>
+   ('VALUE, 'TYPE) EXPRESSION" ("\<lbrakk>_\<rbrakk>\<alpha>\<epsilon>") where
+"EvalAE e = \<epsilon> e"
+
+subsection {* Transfer Theorems *}
+
+theorem EvalAE_simp [evala] :
+"\<lbrakk>e1 \<in> WF_ALPHA_EXPRESSION;
+ e2 \<in> WF_ALPHA_EXPRESSION\<rbrakk> \<Longrightarrow>
+ e1 = e2 \<longleftrightarrow> (\<alpha>\<epsilon> e1) = (\<alpha>\<epsilon> e2) \<and> \<lbrakk>e1\<rbrakk>\<alpha>\<epsilon> = \<lbrakk>e2\<rbrakk>\<alpha>\<epsilon>"
+apply (simp add: EvalAE_def)
+apply (simp add: prod_eq_iff)
+done
+
+theorem EvalAE_intro :
+"\<lbrakk>e1 \<in> WF_ALPHA_EXPRESSION;
+ e2 \<in> WF_ALPHA_EXPRESSION;
+ (\<alpha>\<epsilon> e1) = (\<alpha>\<epsilon> e2);
+ \<lbrakk>e1\<rbrakk>\<alpha>\<epsilon> = \<lbrakk>e2\<rbrakk>\<alpha>\<epsilon> \<rbrakk> \<Longrightarrow> e1 = e2"
+apply (simp add: EvalAE_def)
+apply (simp add: prod_eq_iff)
+done
+
+theorem EvalAE_closure [closure]:
+"e \<in> WF_ALPHA_EXPRESSION \<Longrightarrow>
+\<lbrakk>e\<rbrakk>\<alpha>\<epsilon> \<in> WF_EXPRESSION"
+  by (simp add:WF_ALPHA_EXPRESSION_def WF_EXPRESSION_OVER_def EvalAE_def)
+
+theorem EvalAE_type [typing] :
+"\<lbrakk>e \<in> WF_ALPHA_EXPRESSION; \<epsilon> e :e: t\<rbrakk> \<Longrightarrow> \<lbrakk>e\<rbrakk>\<alpha>\<epsilon> :e: t"
+  by (simp add:EvalAE_def)
+
+theorem EvalAE_tau [simp]: 
+"e \<in> WF_ALPHA_EXPRESSION \<Longrightarrow> \<tau>e \<lbrakk>e\<rbrakk>\<alpha>\<epsilon> = \<tau>e (\<epsilon> e)"
+  by (simp add:EvalAE_def)
+
+subsection {* Distribution Theorems *}
+
+theorem EvalAE_VarAE [evala] :
+"\<lbrakk>VarAE x\<rbrakk>\<alpha>\<epsilon> = VarE x"
+  by (simp add:VarAE_def EvalAE_def)
+
+theorem EvalA_EqualA [evala] :
+"\<lbrakk>e1 \<in> WF_ALPHA_EXPRESSION; 
+ e2 \<in> WF_ALPHA_EXPRESSION\<rbrakk> \<Longrightarrow>
+\<lbrakk>e1 ==\<alpha> e2\<rbrakk>\<pi> = (\<lbrakk>e1\<rbrakk>\<alpha>\<epsilon> ==p \<lbrakk>e2\<rbrakk>\<alpha>\<epsilon>)"
+  by (simp add:EqualA_def EvalA_def EvalAE_def)
+
+theorem EvalE_LitAE [evala] :
+"\<lbrakk>b \<in> WF_BINDING\<rbrakk> \<Longrightarrow>
+ \<lbrakk>LitAE t v\<rbrakk>\<alpha>\<epsilon> = LitE t v"
+  by (simp add: LitAE_def EvalAE_def)
+
+theorem EvalA_SubstA [evala] :
+"\<lbrakk>p \<in> WF_ALPHA_PREDICATE;
+ v \<in> WF_ALPHA_EXPRESSION\<rbrakk> \<Longrightarrow>
+ \<lbrakk>SubstA p v x\<rbrakk>\<pi> = (\<exists>p {x} . \<lbrakk>p\<rbrakk>\<pi> \<and>p ((VarE x) ==p \<lbrakk>v\<rbrakk>\<alpha>\<epsilon>))"
+  apply (simp add:SubstA_def)
+  apply (utp_alpha_tac)
+done
+
+
+theorem EvalA_SubstAE [evala] :
+"\<lbrakk>f \<in> WF_ALPHA_EXPRESSION;
+ v \<in> WF_ALPHA_EXPRESSION\<rbrakk> \<Longrightarrow>
+ \<lbrakk>SubstAE f v x\<rbrakk>\<alpha>\<epsilon> = SubstE \<lbrakk>f\<rbrakk>\<alpha>\<epsilon> \<lbrakk>v\<rbrakk>\<alpha>\<epsilon> x"
+  by (simp add:SubstAE_def EvalAE_def)
+
+subsection {* Proof Experiements *}
+
+theorem SubstAE_VarAE:
+"\<lbrakk>e \<in> WF_ALPHA_EXPRESSION; type x = \<tau>e (\<epsilon> e)\<rbrakk> \<Longrightarrow>
+ SubstAE (VarAE x) e x = e"
+  apply (subgoal_tac "\<epsilon> e :e: type x")
+  apply (utp_alpha_tac)
+  apply (utp_expr_tac)
+  apply (simp add:typing)
+done
+
+end
+end
